\documentclass[11hpt]{article}
\usepackage{amsmath}
\usepackage{mathtools}
\usepackage[all]{xy}
\usepackage{syntax}
\usepackage{trfrac}

\newcommand{\rulelabel}[1]{
\small(\emph{#1})
}

\newcommand{\ruletag}[1]{
  \tag{\emph{#1}}
}

\renewcommand{\syntleft}{\normalfont\itshape}
\renewcommand{\syntright}{}

\begin{document}
\section{All}

\begin{align*}
  \text{lev}_{a,b}(i,j) =
  \begin{cases}
    max(i,j), &min(i,j) = 0 \\
    min
    \begin{cases}
      \text{lev}_{a,b}(i-1,j) + 1 \\
      \text{lev}_{a,b}(i,j-1) + 1 \\
      \text{lev}_{a,b}(i-1,j-1) + (a \neq b)
    \end{cases}
  \end{cases}
\end{align*}

\section{Ambiguity Equations}

\begin{equation*}
  \text{dist}(S_1, S_2) = \frac{\text{lev}(S_1, S_2)}{\text{max}(\text{len}(S_1), \text{len}(S_2))}
\end{equation*}

\begin{align*}
  \text{dist}(S_1, S_2) &= \frac{\text{lev}(S_1, S_2)}{\text{max}(\text{len}(S_1), \text{len}(S_2))} \\
               &= \frac{1}{\text{max}(21, 20)} \\
               &= \frac{1}{21}
\end{align*}

\section{CS Grammar}
\begin{grammar}
<\lambda t> ::= \lit*{() ->} <t>
  \alt \lit*{->} <t>

<v> ::= \lit*{true}
  \alt \lit*{false}
  \alt <\lambda t>

<t> ::= <v>
  \alt <\lambda t>\lit*{()}
  \alt <t> <t>
\end{grammar}

\section{Grammar Examples}

\begin{equation*}
\lambda \lit*{false}\lit*{()}
\end{equation*}

\begin{equation*}
\lambda \lit*{true}  \ \lit*{true}
\end{equation*}

\begin{equation*}
\lambda\lambda \lit*{true}  \lit*{()} \ \lit*{true}
\end{equation*}

\section{Evaluation Rules/Relation}

\begin{equation}
\trfrac[]{}{
  \lambda t \lit*{()} \rightarrow  t
} \ruletag{e-inv}
\end{equation}

\begin{equation}
\trfrac[]{}{
  \lambda t \ v  \rightarrow  t
} \ruletag{e-app}
\end{equation}

\begin{equation}
\trfrac[]{
  t_{2}  \rightarrow  t_{2}'
}{
  t_{1} \  t_{2}  \rightarrow t_{1} \  t_{2}'
} \ruletag{e-arg-eval}
\end{equation}

\begin{equation}
\trfrac[]{
   t \rightarrow  t'
}{
  t \ v \rightarrow t' \ v
} \ruletag{e-app-eval}
\end{equation}

\begin{equation*}
\trfrac[\rulelabel{e-inv}]{
}{
  \lambda \lit*{false} \lit*{()} \to \lit*{false}
}
\end{equation*}

\begin{equation*}
\trfrac[\rulelabel{e-app-eval}]{
  \trfrac[\rulelabel{e-inv}]{}{
    \lambda \lambda \lit*{true} \lit*{()} \to \lambda \lit*{true}
  }
}{
  \lambda \lambda \lit*{true} \lit*{()}\ \lit*{true}  \to \lambda \lit*{true}\ \lit*{true}
}
\begin{equation*}

\begin{equation*}
\trfrac[\rulelabel{e-app}]{}{
  \lambda \lit*{true}\ \lit*{true} \to \lit*{true}
}
\begin{equation*}

\begin{equation*}
( \lit*{(-> true)()},\ \trfrac[\rulelabel{e-inv}]{}{\lambda \lit*{true()} \to \lit*{true}},\ Bool)

\end{equation*}

\end{document}